\documentclass{article}

\usepackage{amsmath}

\begin{document}

\title{Conditional Random Fields}

\maketitle

% ==========================================
% Beginning of text.                       |
% ==========================================

\section{Introduction}

Let $ x = \{x_1, x_2, ..., x_n \} $ be a sequence of tokens and $ y = \{y_1, y_2, ..., y_n \} $ 
a sequence of labels attributed to these tokens. Let the conditional probability of $ y $ be 
defined by:

\begin{equation}
P(y|x) = \frac{1}{Z(x)} \prod_{t=1}^{T}exp\left\{\sum_{k=1}^{K} \theta_k f_k(y_t, y_{t-1}, x_t)\right\}
\label{eq:1}
\end{equation}

The partition function is given by:

\begin{equation}
Z(x) = \sum_{y'}\prod_{t=1}^{T}exp\left\{\sum_{k=1}^{K} \theta_k f_k(y'_t, y'_{t-1}, x_t)\right\}
\label{eq:2}
\end{equation}

$ P(y|x; \theta) $ is the conditional likelihood $ \mathcal{L}(\theta) $. And the log conditional likelihood
is given by:

\begin{equation}
\begin{split}
\ell(\theta) & = log \prod_{t=1}^{T}exp\left\{\sum_{k=1}^{K} \theta_k f_k(y_t, y_{t-1}, x_t)\right\} - log Z(x) \\
             & = \sum_{t=1}^{T}\sum_{k=1}^{K} \theta_k f_k(y_t, y_{t-1}, x_t) - log Z(x)
\end{split}
\label{eq:3}
\end{equation}

Now we want to obtain the feature parameters $ \theta $ by maximum likelihood. For that, we need to find the
derivative of $ ell(\theta) $ relative to each parameter.

\begin{equation}
\frac{\partial \ell(\theta)}{\partial \theta_k} = \sum_{t=1}^{T}\sum_{k=1}^{K} f_k(y_t, y_{t-1}, x_t) - \frac{\partial log Z(x)}{\partial \theta_k}
\label{eq:4}
\end{equation}

\begin{equation}
\frac{\partial log Z(x)}{\partial \theta_k} = \frac{1}{Z(x)}\frac{\partial Z(x)}{\partial \theta_k}
\label{eq:5}
\end{equation}

\begin{equation}
\frac{\partial Z(x)}{\partial \theta_k} = \sum_{y'}\frac{\partial}{\partial \theta_k} \prod_{t=1}^{T}exp\left\{\sum_{k=1}^{K} \theta_k f_k(y'_t, y'_{t-1}, x_t)\right\}
\label{eq:6}
\end{equation}

\begin{equation}
\frac{\partial}{\partial \theta_k} \prod_{t=1}^{T}exp\left\{\sum_{k=1}^{K} \theta_k f_k(y'_t, y'_{t-1}, x_t)\right\} = 
\frac{\partial}{\partial \theta_k} exp\left\{\sum_{t=1}^{T}\sum_{k=1}^{K} \theta_k f_k(y'_t, y'_{t-1}, x_t)\right\}
\label{eq:7}
\end{equation}

\begin{equation}
\frac{\partial}{\partial \theta_k} exp\left\{\sum_{t=1}^{T}\sum_{k=1}^{K} \theta_k f_k(y'_t, y'_{t-1}, x_t)\right\} = 
exp\left\{\sum_{t=1}^{T}\sum_{k=1}^{K} \theta_k f_k(y'_t, y'_{t-1}, x_t)\right\} \sum_{t=1}^{T}f_k(y'_t, y'_{t-1}, x_t)
\label{eq:8}
\end{equation}

\begin{equation}
\frac{\partial log Z(x)}{\partial \theta_k} = \frac{1}{Z(x)}\sum_{y'}
\prod_{t=1}^{T} exp\left\{\sum_{k=1}^{K} \theta_k f_k(y'_t, y'_{t-1}, x_t)\right\} \sum_{t=1}^{T}f_k(y'_t, y'_{t-1}, x_t)
\label{eq:9}
\end{equation}

\begin{equation}
\frac{\partial log Z(x)}{\partial \theta_k} = \sum_{y'}
\frac{\prod_{t=1}^{T} exp\left\{\sum_{k=1}^{K} \theta_k f_k(y'_t, y'_{t-1}, x_t)\right\}}{\sum_{y''}\prod_{t=1}^{T}exp\left\{\sum_{k=1}^{K} f_k(y''_t, y''_{t-1}, x_t)\right\}}
\sum_{t=1}^{T}\theta_k f_k(y'_t, y'_{t-1}, x_t)
\label{eq:10}
\end{equation}

\begin{equation}
\frac{\partial log Z(x)}{\partial \theta_k} = \sum_{y'} P(y'|x) \sum_{t=1}^{T}f_k(y'_t, y'_{t-1}, x_t)
\label{eq:11}
\end{equation}

\begin{equation}
\frac{\partial log Z(x)}{\partial \theta_k} =  \sum_{t=1}^{T}\sum_{y'} f_k(y'_t, y'_{t-1}, x_t) P(y'|x)
\label{eq:12}
\end{equation}

\begin{equation}
\frac{\partial log Z(x)}{\partial \theta_k} =  \sum_{t=1}^{T}\sum_{y, y'} f_k(y, y', x_t) P(y, y'|x)
\label{eq:13}
\end{equation}

Essa parte demanda explicação!!!!

% ==========================================
% End of text.                             |
% ==========================================

\end{document}
